#### Question 6: `Use the chain rule to compute the derivative df/dx of the aforementioned function, placing each term on the dependency graph that you constructed previously.`

$$
f(x) = \left( \log(x^2) \cdot \sin x \right) + x^{-1}
$$

---

### **1. Recall the intermediate steps (dependencies)**

We'll reuse these:

| Variable | Expression  |
| -------- | ----------- |
| a        | $x^2$       |
| b        | $\log(a)$   |
| c        | $\sin(x)$   |
| d        | $b \cdot c$ |
| e        | $x^{-1}$    |
| f        | $d + e$     |

---

### **2. Derivatives of each node using the chain rule**

Let’s compute the derivatives step-by-step.

---

#### **$a = x²$**

$$
\frac{da}{dx} = 2x
$$

---

#### **$b = log(a)$**

$$
\frac{db}{dx} = \frac{db}{da} \cdot \frac{da}{dx} = \frac{1}{a} \cdot 2x = \frac{2x}{x^2} = \frac{2}{x}
$$

---

#### **$c = sin(x)$**

$$
\frac{dc}{dx} = \cos(x)
$$

---

#### **$d = b \cdot c$**

Apply the product rule:

$$
\frac{dd}{dx} = \frac{db}{dx} \cdot c + b \cdot \frac{dc}{dx} = \frac{2}{x} \cdot \sin(x) + \log(x^2) \cdot \cos(x)
$$

---

#### **$e = x^{-1}$**

$$
\frac{de}{dx} = \frac{d}{dx}(x^{-1}) = -x^{-2}
$$

---

#### **$f = d + e$**

$$
\frac{df}{dx} = \frac{dd}{dx} + \frac{de}{dx}
$$

Putting everything together:

$$
\frac{df}{dx} = \frac{2}{x} \cdot \sin(x) + \log(x^2) \cdot \cos(x) - \frac{1}{x^2}
$$

---

### **3. Annotated Dependency Graph with Derivatives**

```text
         x
       / | \
      /  |  \
     /   |   \
 x^2   sin(x)  x⁻¹
  |      |      |
  |      |      |
 da/dx=2x  dc/dx=cos(x)  de/dx=−1/x²
  |      |      |
 log     |      |
  |      |      |
 db/dx=(1/a)(da/dx)=2/x
   \    /       
    \  /        
   (·)          
    |           
 dd/dx = (2/x)·sin(x) + log(x²)·cos(x)
     \         
      \       
       \     
        (+)
          |
    df/dx = dd/dx + de/dx
          = (2/x)·sin(x) + log(x²)·cos(x) − 1/x²
```

---

###  Final Derivative:

$$
\boxed{
\frac{df}{dx} = \frac{2}{x} \cdot \sin(x) + \log(x^2) \cdot \cos(x) - \frac{1}{x^2}
}
$$




